Also use EnvMaps in RemoveParams, optimizing it some more

erasure/src/pCUICWcbvEval.ml
@@ -1,0 +1,28 @@
+open BasicAst
+open Datatypes
+open PCUICAst
+open Universes0
+
+type eval =
+| Coq_eval_beta of term * aname * term * term * term * term * term * 
+   eval * eval * eval
+| Coq_eval_zeta of aname * term * term * term * term * term * eval * eval
+| Coq_eval_delta of kername * PCUICEnvironment.constant_body * term
+   * Instance.t * term * eval
+| Coq_eval_iota of case_info * term * nat
+   * PCUICEnvironment.mutual_inductive_body
+   * PCUICEnvironment.one_inductive_body * PCUICEnvironment.constructor_body
+   * Instance.t * term list * term predicate * term branch list * term branch
+   * term * eval * eval
+| Coq_eval_proj of inductive * nat * nat * term * term list * Instance.t
+   * term * term * eval * eval
+| Coq_eval_fix of term * term mfixpoint * nat * term list * term * term
+   * term * term * eval * eval * eval
+| Coq_eval_fix_value of term * term mfixpoint * nat * term list * term * 
+   term * nat * term * eval * eval
+| Coq_red_cofix_case of case_info * term mfixpoint * nat * term predicate
+   * term list * nat * term * term branch list * term * eval
+| Coq_red_cofix_proj of projection * term mfixpoint * nat * term list * 
+   nat * term * term * eval
+| Coq_eval_app_cong of term * term * term * term * eval * eval
+| Coq_eval_atom of term
