erasure/theories/Erasure.v
@@ -28,9 +28,6 @@ Extract Constant time => "(fun c f x -> let s = Tm_util.list_to_string c in Tm_u
   shrinking of the global environment dependencies +
   the optimization that removes all pattern-matches on propositions. *)
 
-Definition eprogram := 
-  (EAst.global_context * EAst.term).
-
 Import EOptimizePropDiscr.
 
 Module Transform.
@@ -99,16 +96,22 @@ Module Transform.
 End Transform.
 Import ETyping.
 
-Definition self_optimization program value eval eval' := Transform.t program program value value eval eval'.
+Definition self_transform program value eval eval' := Transform.t program program value value eval eval'.
+
+Definition eprogram := 
+  (EAst.global_context * EAst.term).
+
+Import ERemoveParams.GlobalContextMap (make, global_decls).
 
 Definition eval_eprogram (wfl : EWcbvEval.WcbvFlags) (p : eprogram) (t : EAst.term) := 
   EWcbvEval.eval (wfl:=wfl) p.1 p.2 t.
 
 Import Transform.
 Obligation Tactic := idtac.
-Program Definition optimize_prop_discr_optimization : self_optimization eprogram EAst.term (eval_eprogram EWcbvEval.default_wcbv_flags) (eval_eprogram EWcbvEval.opt_wcbv_flags) := 
+Program Definition optimize_prop_discr_optimization : self_transform eprogram EAst.term (eval_eprogram EWcbvEval.default_wcbv_flags) (eval_eprogram EWcbvEval.opt_wcbv_flags) := 
   {| name := "optimize_prop_discr"; 
-    transform p _ := (EOptimizePropDiscr.optimize_env p.1, EOptimizePropDiscr.optimize p.1 p.2);
+    transform p _ := 
+      (EOptimizePropDiscr.optimize_env p.1, EOptimizePropDiscr.optimize p.1 p.2);
     pre p := (closed_env p.1 /\ ELiftSubst.closedn 0 p.2);
     post p := (closed_env p.1 /\ ELiftSubst.closedn 0 p.2);
     obseq g g' v v' := v' = EOptimizePropDiscr.optimize g.1 v
@@ -128,10 +131,29 @@ Next Obligation.
   eapply EOptimizePropDiscr.optimize_correct in ev; eauto.
 Qed.
 
-Program Definition remove_params_optimization (fl : EWcbvEval.WcbvFlags) : self_optimization eprogram EAst.term (eval_eprogram fl) (eval_eprogram fl) :=
+Lemma wf_glob_fresh Σ : wf_glob Σ -> EnvMap.EnvMap.fresh_globals Σ.
+Proof.
+  induction Σ. constructor; auto.
+  intros wf; depelim wf. constructor; auto.
+Qed.
+
+Definition eprogram_env := 
+  (ERemoveParams.GlobalContextMap.t * EAst.term).
+
+Definition eval_eprogram_env (wfl : EWcbvEval.WcbvFlags) (p : eprogram_env) (t : EAst.term) := 
+  EWcbvEval.eval (wfl:=wfl) p.1.(global_decls) p.2 t.
+
+Program Definition remove_params (p : eprogram_env) : eprogram :=
+  (ERemoveParams.strip_env p.1, ERemoveParams.strip p.1 p.2).
+
+Program Definition remove_params_optimization (fl : EWcbvEval.WcbvFlags) : 
+  Transform.t eprogram_env eprogram EAst.term EAst.term (eval_eprogram_env fl) (eval_eprogram fl) :=
   {| name := "remove_parameters";
-    transform p _ := (ERemoveParams.strip_env p.1, ERemoveParams.strip p.1 p.2);
-    pre p := [/\ wf_glob p.1, ERemoveParams.isEtaExp_env p.1, ERemoveParams.isEtaExp p.1 p.2, closed_env p.1 & ELiftSubst.closedn 0 p.2];
+    transform p pre := remove_params p;
+    pre p := 
+    let decls := p.1.(global_decls) in
+     [/\ wf_glob decls, ERemoveParams.isEtaExp_env decls, 
+      ERemoveParams.isEtaExp decls p.2, closed_env decls & ELiftSubst.closedn 0 p.2];
     post p := (closed_env p.1 /\ ELiftSubst.closedn 0 p.2);
     obseq g g' v v' := v' = (ERemoveParams.strip g.1 v) |}.
 Next Obligation.
@@ -140,10 +162,9 @@ Next Obligation.
   cbn -[ERemoveParams.strip] in *.
   split.
   move: cle. unfold closed_env. unfold ERemoveParams.strip_env.
-  induction Σ at 1 3; cbn; auto.
-  move/andP => [] cla clg. rewrite (IHg clg) andb_true_r.
-  destruct a as [kn []]; cbn in * => //.
-  destruct E.cst_body => //. cbn -[ERemoveParams.strip] in cla |- *.
+  rewrite forallb_map. eapply forallb_impl. intros.
+  destruct x as [kn []]; cbn in * => //.
+  destruct E.cst_body => //. cbn -[ERemoveParams.strip] in H0 |- *.
   now eapply ERemoveParams.closed_strip.
   now eapply ERemoveParams.closed_strip.
 Qed.
@@ -152,11 +173,14 @@ Next Obligation.
   eapply ERemoveParams.strip_eval in ev; eauto.
 Qed.
 
-
-Program Definition remove_params_fast_optimization (fl : EWcbvEval.WcbvFlags) : self_optimization eprogram EAst.term (eval_eprogram fl) (eval_eprogram fl) :=
+Program Definition remove_params_fast_optimization (fl : EWcbvEval.WcbvFlags) :
+  Transform.t eprogram_env eprogram EAst.term EAst.term (eval_eprogram_env fl) (eval_eprogram fl) :=
   {| name := "remove_parameters_fast";
     transform p _ := (ERemoveParams.Fast.strip_env p.1, ERemoveParams.Fast.strip p.1 [] p.2);
-    pre p := [/\ wf_glob p.1, ERemoveParams.isEtaExp_env p.1, ERemoveParams.isEtaExp p.1 p.2, closed_env p.1 & ELiftSubst.closedn 0 p.2];
+    pre p := 
+      let decls := p.1.(global_decls) in
+      [/\ wf_glob decls, ERemoveParams.isEtaExp_env decls, 
+       ERemoveParams.isEtaExp decls p.2, closed_env decls & ELiftSubst.closedn 0 p.2];
     post p := (closed_env p.1 /\ ELiftSubst.closedn 0 p.2);
     obseq g g' v v' := v' = (ERemoveParams.strip g.1 v) |}.
 Next Obligation.
@@ -166,10 +190,9 @@ Next Obligation.
   cbn -[ERemoveParams.strip] in *.
   split.
   move: cle. unfold closed_env. unfold ERemoveParams.strip_env.
-  induction Σ at 1 3; cbn; auto.
-  move/andP => [] cla clg. rewrite (IHg clg) andb_true_r.
-  destruct a as [kn []]; cbn in * => //.
-  destruct E.cst_body => //. cbn -[ERemoveParams.strip] in cla |- *.
+  rewrite forallb_map. eapply forallb_impl. intros.
+  destruct x as [kn []]; cbn in * => //.
+  destruct E.cst_body => //. cbn -[ERemoveParams.strip] in H0 |- *.
   now eapply ERemoveParams.closed_strip.
   now eapply ERemoveParams.closed_strip.
 Qed.
@@ -177,37 +200,119 @@ Next Obligation.
   red. move=> [Σ t] /= v [wfe etae etat cle clt] ev.
   rewrite -ERemoveParams.Fast.strip_fast -ERemoveParams.Fast.strip_env_fast.
   eapply ERemoveParams.strip_eval in ev; eauto.
+Qed.
+
+Definition pcuic_program := 
+  global_env_ext_map * term.
+
+Definition eval_program (p : Ast.Env.program) (v : Ast.term) :=
+  WcbvEval.eval p.1 p.2 v.  
+  
+Definition eval_pcuic_program (p : pcuic_program) (v : term) :=
+  PCUICWcbvEval.eval p.1.(trans_env_env) p.2 v.
+
+Definition template_to_pcuic_obseq (p : Ast.Env.program) (p' : pcuic_program) (v : Ast.term) (v' : term) :=
+  let Σ := Ast.Env.empty_ext p.1 in v' = trans (trans_global Σ) v.
+  
+Program Definition template_to_pcuic_transform {cf : checker_flags} : 
+  Transform.t Ast.Env.program pcuic_program Ast.term term 
+  eval_program eval_pcuic_program :=
+ {| name := "template to pcuic";
+    pre p :=  
+      let Σ := Ast.Env.empty_ext p.1 in
+      ∥ Typing.wf_ext Σ × ∑ T, Typing.typing (Ast.Env.empty_ext p.1) [] p.2 T ∥;
+    transform p hp := let Σ' := trans_global (Ast.Env.empty_ext p.1) in 
+      (Σ', trans Σ' p.2) ;
+    post p := ∥ wf_ext p.1 × ∑ T, typing p.1 [] p.2 T ∥;
+    obseq := template_to_pcuic_obseq |}.
+Next Obligation.
+  intros cf [Σ t] [[wfext ht]].
+  set (Σ' := trans_global _).
+  cbn. sq. split => //. eapply template_to_pcuic_env_ext. apply wfext.
+  destruct ht as [T HT]. exists (trans (trans_global_env Σ) T).
+  eapply (template_to_pcuic_typing (Σ := Ast.Env.empty_ext Σ) []). apply wfext.
+  apply HT.
+Qed.
+Next Obligation.
+  red. intros cf [Σ t] v [[]].
+  unfold eval_pcuic_program, eval_program.
+  cbn. intros ev.
+  unshelve eapply TemplateToPCUICWcbvEval.trans_wcbvEval in ev; eauto. apply w.
+  eexists; split; split; eauto. red. reflexivity.
+  eapply template_to_pcuic_env.
+  apply w. destruct s as [T HT]. apply TypingWf.typing_wf in HT. apply HT. auto.
+Qed.
+
+Program Definition build_global_env_map (g : global_env) : global_env_map := 
+  {| trans_env_env := g; 
+     trans_env_map := EnvMap.EnvMap.of_global_env g.(declarations) |}.
+Next Obligation.
+  intros g. eapply EnvMap.EnvMap.repr_global_env.
+Qed.
+
+Definition let_expansion_obseq (p : pcuic_program) (p' : pcuic_program) (v : term) (v' : term) :=
+  v' = PCUICExpandLets.trans v.
+
+Program Definition pcuic_expand_lets_transform {cf : checker_flags} : 
+  self_transform pcuic_program term eval_pcuic_program eval_pcuic_program :=
+ {| name := "let expansion in branches/constructors";
+    pre p :=
+      let Σ : global_env_ext := p.1 in
+      ∥ wf_ext Σ × ∑ T, typing Σ nil p.2 T ∥;
+    transform p hp := 
+      let Σ' := PCUICExpandLets.trans_global p.1 in 
+      ((build_global_env_map Σ', p.1.2), PCUICExpandLets.trans p.2) ;
+    post p := ∥ wf_ext (H:=PCUICExpandLetsCorrectness.cf' cf) p.1 × 
+      ∑ T, typing (H:=PCUICExpandLetsCorrectness.cf' cf) p.1 nil p.2 T ∥;
+    obseq := let_expansion_obseq |}.
+Next Obligation.
+  intros cf [Σ t] [[wfext ht]].
+  set (Σ' := PCUICExpandLets.trans_global _).
+  cbn. sq. unfold build_global_env_map. unfold global_env_ext_map_global_env_ext. simpl.
+  split. eapply PCUICExpandLetsCorrectness.trans_wf_ext in wfext. apply wfext.
+  destruct ht as [T HT]. exists (PCUICExpandLets.trans T).
+  eapply (PCUICExpandLetsCorrectness.pcuic_expand_lets Σ []) => //.
+  apply wfext. apply PCUICExpandLetsCorrectness.trans_wf_ext in wfext. apply wfext.
+Qed.
+Next Obligation.
+  red. intros cf [Σ t] v [[]].
+  unfold eval_pcuic_program.
+  cbn. intros ev.
+  unshelve eapply (PCUICExpandLetsCorrectness.trans_wcbveval (Σ:=Σ)) in ev; eauto.
+  eexists; split; split; eauto. red. reflexivity.
+  destruct s as [T HT]. now apply PCUICClosedTyp.subject_closed in HT.
 Qed.
 
 Obligation Tactic := program_simpl.
-Program Definition erase_template_program (p : Ast.Env.program) univs 
-  (wfΣ : ∥ Typing.wf_ext (p.1, univs) ∥)
-  (wt : ∥ ∑ T, Typing.typing (p.1, univs) [] p.2 T ∥)
-  : eprogram :=
-  let Σ0 := (trans_global (Ast.Env.empty_ext p.1)).1 in
-  let Σ := (PCUICExpandLets.trans_global_env Σ0) in
-  let wfΣ := map_squash (PCUICExpandLetsCorrectness.trans_wf_ext ∘
-    (template_to_pcuic_env_ext (p.1, univs))) wfΣ in
-  let wfe := build_wf_env _ (map_squash (wf_ext_wf _) wfΣ) in
-  let wfe' := make_wf_env_ext wfe univs wfΣ in
-  let t := ErasureFunction.erase wfe' nil (PCUICExpandLets.trans (trans Σ0 p.2)) _ in
+
+Definition build_wf_env_from_env {cf : checker_flags} (Σ : global_env_map) (wfΣ : ∥ wf Σ ∥) : wf_env := 
+  {| wf_env_env := Σ.(trans_env_env);
+     wf_env_map := Σ.(trans_env_map);
+     wf_env_map_repr := Σ.(trans_env_repr);
+     wf_env_wf := wfΣ;
+     wf_env_graph := (graph_of_wf wfΣ).π1;
+     wf_env_graph_wf := (graph_of_wf wfΣ).π2 |}.
+
+Program Definition erase_pcuic_program (p : pcuic_program) 
+  (wfΣ : ∥ wf_ext (H := config.extraction_checker_flags) p.1 ∥)
+  (wt : ∥ ∑ T, typing (H := config.extraction_checker_flags) p.1 [] p.2 T ∥) : eprogram_env :=
+  let wfe := build_wf_env_from_env p.1.1 (map_squash (wf_ext_wf _) wfΣ) in
+  let wfe' := make_wf_env_ext wfe p.1.2 wfΣ in
+  let t := ErasureFunction.erase wfe' nil p.2 _ in
   let Σ' := ErasureFunction.erase_global (term_global_deps t) wfe in
-  (Σ', t).
+  (ERemoveParams.GlobalContextMap.make Σ' _, t).
   
 Next Obligation.
   sq. destruct wt as [T Ht].
-  cbn.
-  set (Σ' := (_, univs)).
-  exists (PCUICExpandLets.trans (trans (trans_global_env p.1) T)).
-  change Σ' with (PCUICExpandLets.trans_global (trans_global (p.1, univs))).
-  change (@nil (@BasicAst.context_decl term)) with (PCUICExpandLets.trans_local (trans_local (trans_global_env p.1) [])).
-  change (trans_global_env p.1) with (global_env_ext_map_global_env_map (trans_global (p.1, univs))).
-  eapply (@PCUICExpandLetsCorrectness.expand_lets_sound (extraction_checker_flags)).
-  now eapply template_to_pcuic_env.
-  now eapply template_to_pcuic_typing.
-Defined.
+  cbn. now exists T.
+Qed.
+Next Obligation.
+  unfold erase_global.
+  eapply wf_glob_fresh.
+  eapply ERemoveParams.erase_global_decls_wf_glob.
+Qed.
 
-(** The full correctness lemma of erasure from Template programs do λ-box *)
+(* * The full correctness lemma of erasure from Template programs do λ-box
 
 Lemma erase_template_program_correctness {p : Ast.Env.program} univs
   (Σ := (p.1, univs))
@@ -256,62 +361,67 @@ Proof.
   destruct H as [v' [Hv He]].
   sq.
   set (eΣ := erase_global _ _) in *. exists v'. split => //.
-Qed.
-
-Definition eval_program (p : Ast.Env.program) (v : Ast.term) :=
-  WcbvEval.eval p.1 p.2 v.
+Qed. *)
 
 Obligation Tactic := idtac.
 
-Program Definition erase_transform : Transform.t Ast.Env.program eprogram Ast.term EAst.term eval_program (eval_eprogram EWcbvEval.default_wcbv_flags) :=
+Program Definition erase_transform : Transform.t pcuic_program eprogram_env term EAst.term eval_pcuic_program (eval_eprogram_env EWcbvEval.default_wcbv_flags) :=
  {| name := "erasure";
     pre p :=  
-      let Σ := Ast.Env.empty_ext p.1 in
-      ∥ Typing.wf_ext Σ × ∑ T, Typing.typing (Ast.Env.empty_ext p.1) [] p.2 T ∥;
-    transform p hp := erase_template_program p Monomorphic_ctx (map_squash fst hp) (map_squash snd hp) ;
-    post p := (wf_glob p.1 /\ closed_env p.1 /\ ELiftSubst.closedn 0 p.2);
-    obseq g g' v v' :=
-      let Σ := Ast.Env.empty_ext g.1 in
-      PCUICExpandLets.trans_global (trans_global Σ) ;;; [] |- 
-      PCUICExpandLets.trans (trans (trans_global Σ) v) ⇝ℇ v' /\ 
-      ∥ EWcbvEval.eval (wfl:=EWcbvEval.default_wcbv_flags) g'.1 g'.2 v' ∥ |}.
+      ∥ wf_ext (H := config.extraction_checker_flags) p.1 × ∑ T, typing (H := config.extraction_checker_flags) p.1 [] p.2 T ∥;
+    transform p hp := erase_pcuic_program p (map_squash fst hp) (map_squash snd hp) ;
+    post p :=
+      let decls := p.1.(global_decls) in
+      [/\ wf_glob decls, closed_env decls & ELiftSubst.closedn 0 p.2];
+    obseq g g' v v' := let Σ := g.1 in Σ ;;; [] |- v ⇝ℇ v' |}.
 Next Obligation.
   intros [Σ t] [[wfext ht]].
-  destruct erase_template_program eqn:e.
-  unfold erase_template_program in e. simpl. injection e. intros <- <-. split.
-  eapply ERemoveParams.erase_global_wf_glob. split.
+  destruct erase_pcuic_program eqn:e.
+  unfold erase_pcuic_program in e. simpl. injection e. intros <- <-. split.
+  eapply ERemoveParams.erase_global_wf_glob.
   eapply erase_global_closed.
   eapply (erases_closed _ []). 2:eapply erases_erase.
   clear e. destruct ht as [T HT].
-  eapply (template_to_pcuic_typing []) in HT; eauto.
-  simpl in HT.
-  eapply (@PCUICClosedTyp.subject_closed _ _) in HT.
-  now eapply PCUICExpandLetsCorrectness.trans_closedn.
-  now eapply template_to_pcuic_env_ext.
+  now eapply (@PCUICClosedTyp.subject_closed _ _) in HT.
 Qed.
 Next Obligation.
-  red. move=> [Σ t] v [[wf [T HT]]]. unfold eval_program.
+  red. move=> [Σ t] v [[wf [T HT]]]. unfold eval_pcuic_program, eval_eprogram.
   intros ev.
-  destruct erase_template_program eqn:e.
-  eapply (erase_template_program_correctness) in e; tea.
-  destruct e as [v' [he [hev]]]. exists v'; split; split => //.
+  destruct erase_pcuic_program eqn:e.
+  unfold erase_pcuic_program in e. simpl in e. injection e; intros <- <-.
+  simpl. clear e. cbn in *.
+  set (Σ' := build_wf_env_from_env _ _).
+  (* assert (wt : PCUICSafeLemmata.welltyped (cf:=config.extraction_checker_flags) Σ [] t). now exists T. *)
+  eapply (erase_correct Σ' Σ.2 _ _ _ _ _ (term_global_deps _)) in ev; try reflexivity.
+  2:eapply Kernames.KernameSet.subset_spec; reflexivity.
+  destruct ev as [v' [he [hev]]]. exists v'; split; split => //.
+  red. cbn.
+  eexact hev.
 Qed.
 
 Obligation Tactic := program_simpl.
+
+Local Notation " o ▷ o' " := (Transform.compose o o' _) (at level 50, left associativity).
+
 Program Definition erasure_pipeline := 
-  Transform.compose erase_transform 
-  (Transform.compose (remove_params_optimization _)
-    optimize_prop_discr_optimization _) _.
+  template_to_pcuic_transform ▷
+  pcuic_expand_lets_transform ▷
+  erase_transform ▷ 
+  remove_params_optimization _ ▷ 
+  optimize_prop_discr_optimization.
+
 Next Obligation.
-  split => //. all:todo "etaexp".
+  sq. split => //. all:todo "etaexp".
 Qed.
 
 Definition erase_program := run erasure_pipeline.
 
 Program Definition erasure_pipeline_fast := 
-  Transform.compose erase_transform 
-  (Transform.compose (remove_params_fast_optimization _)
-    optimize_prop_discr_optimization _) _.
+  template_to_pcuic_transform ▷
+  pcuic_expand_lets_transform ▷
+  erase_transform ▷ 
+  remove_params_fast_optimization _ ▷ 
+  optimize_prop_discr_optimization.
 Next Obligation.
   split => //. all:todo "etaexp".
 Qed.
