test-suite/self_erasure.v
@@ -1,7 +1,7 @@
 From MetaCoq.Erasure Require Import Loader Erasure.
 From MetaCoq.SafeChecker Require Import PCUICSafeChecker.
 Set MetaCoq Timing.
-(* 1sec *)
+(* <1sec *)
 MetaCoq Fast Erase @erase_and_print_template_program.
-(* 4sec *)
-Time MetaCoq Erase @typecheck_program.
+(* 2sec *)
+MetaCoq Fast Erase @typecheck_program.
